redefine notion of buffer equivalence during compact to use interpretation function I() that interprets a BufferStack to a Buffer

Splinter/Betree/BufferStack.i.dfy
@@ -25,6 +25,12 @@ module BufferStackMod
       BufferStack(buffers[start..end])
     }
 
+    function DropFirst() : BufferStack
+      requires 0 < |buffers|
+    {
+      Slice(1, |buffers|)
+    }
+
     function QueryUpTo(key: Key, count: nat) : Message
       requires count <= |buffers|
     {
@@ -50,6 +56,60 @@ module BufferStackMod
     predicate Equivalent(other: BufferStack)
     {
       forall k | AnyKey(k) :: Query(k) == other.Query(k)
+    }
+
+    function IBottom(offsetMap: OffsetMap) : Buffer 
+      requires offsetMap.WF()
+      requires 0 < |buffers|
+    {
+      buffers[0].ApplyFilter(offsetMap.FilterForBottom())
+    }
+
+    function I(offsetMap: OffsetMap) : Buffer 
+      requires offsetMap.WF()
+      decreases |buffers|
+    {
+      if |buffers| == 0 then EmptyBuffer()
+      else DropFirst().I(offsetMap.Decrement(1)).Merge(IBottom(offsetMap))
+    }
+  }
+
+
+  // TotalMapMod provides something like these, but it depends on module
+  // refinement that's hairy and has problems in use (rank_is_less_than doesn't
+  // make it through the module refinement, so we can't prove decreases).
+  predicate AnyKey(key: Key) { true }
+  predicate Total(keys: iset<Key>) {
+    forall k | AnyKey(k) :: k in keys
+  }
+  function AllKeys() : (out: iset<Key>)
+    ensures Total(out)
+  {
+    iset k | AnyKey(k)
+  }
+
+  datatype OffsetMap = OffsetMap(offsets: imap<Key, nat>)
+  {
+    predicate WF() {
+      Total(offsets.Keys)
+    }
+
+    function Get(k: Key) : nat 
+      requires WF()
+    {
+      offsets[k]
+    }
+
+    function FilterForBottom() : iset<Key> 
+      requires WF()
+    {
+      iset k | offsets[k] == 0
+    }
+
+    function Decrement(i: nat) : OffsetMap 
+      requires WF()
+    {
+      OffsetMap(imap k | AnyKey(k) :: if i <= offsets[k] then offsets[k]-i else 0)
     }
   }
 }
